\subsection{Grundlagen}\label{grundlagen}
\chead{LÃ¶sungen -- Grundlagen}

\subsubsection{Terme addieren, subtrahieren und multiplizieren}

\begin{aufgaben}
\item $3 x^2-4 x-4 +  x-2 = 3 x^2-3 x-6$
\item $7 x^2+4 x-6 +  x^2-11 x+13 = 8 x^2-7 x+7$
\item $6 x^2-2 x-1 + \big(-4 x^2+7 x+5\big) = 2 x^2+5 x+4$ \\
\hrule
\item $3 x^3+4 x^2 - \big(2 x^3+3\big) =  x^3+4 x^2-3$
\item $5 x^3+9 x+4 - \big(9 x-4\big) = 5 x^3+8$
\item $7 x^2-9 x+2 - \big(7 x^3+9 x^2-2 x\big) = -7 x^3-2 x^2-7 x+2$
\item $4 x^2-3 x+2 - \big(- x^2-3 x\big) = 5 x^2+2$
\item $8 x^2-6 x+2 - \big(3 x^2+7 x-4\big) = 5 x^2-13 x+6$ \\
\hrule
\item $\big(7 x+3\big) \cdot \big( x-3\big) = 7 x^2-18 x-9$ \\
\item $\big(9 x-1\big) \cdot \big(9 x+1\big) = 81 x^2-1$ \\
\item $\big( x^2+6\big) \cdot \big(-2 x^2+7\big) = -2 x^4-5 x^2+42$ \\
\item $\big( 1+x\big) \cdot \big( x^2-5 x-6\big) =  x^3-4 x^2-11 x-6$ \\
\item $\big( x^2-3\big) \cdot \big(3 x^3-5 x^2+2 x-1\big) = 3 x^5-5 x^4-7 x^3+14 x^2-6 x+3$
\end{aufgaben}

\subsubsection{Potenzgesetze anwenden}

\begin{aufgaben}
\item $x^9\cdot x^5=x^{15}$
\item $x^7\cdot x^2=x^9$
\hrule
\item $x^7:x^5 = x^2$
\item $x^{12}:x^{8}=x^4$
\hrule
\item $\dfrac{x\cdot x\cdot x\cdot x\cdot x\cdot x\cdot x}{x\cdot x}=x^5$
\end{aufgaben}